src/arch/x64/X64.Vale.QuickCodes_i.fsti
@@ -156,12 +156,12 @@ let qInlineIf (#a:Type) (#c1:code) (#c2:code) (b:bool) (qc1:quickCode a c1) (qc2
   QProc (if_code b c1 c2) (wp_InlineIf b qc1 qc2) (qInlineIf_monotone b qc1 qc2) (qInlineIf_compute b qc1 qc2) (qInlineIf_proof b qc1 qc2)
 
 type cmp =
-| Cmp_eq : operand -> operand -> cmp
-| Cmp_ne : operand -> operand -> cmp
-| Cmp_le : operand -> operand -> cmp
-| Cmp_ge : operand -> operand -> cmp
-| Cmp_lt : operand -> operand -> cmp
-| Cmp_gt : operand -> operand -> cmp
+| Cmp_eq : o1:operand{not (OMem? o1)} -> o2:operand{not (OMem? o2)} -> cmp
+| Cmp_ne : o1:operand{not (OMem? o1)} -> o2:operand{not (OMem? o2)} -> cmp
+| Cmp_le : o1:operand{not (OMem? o1)} -> o2:operand{not (OMem? o2)} -> cmp
+| Cmp_ge : o1:operand{not (OMem? o1)} -> o2:operand{not (OMem? o2)} -> cmp
+| Cmp_lt : o1:operand{not (OMem? o1)} -> o2:operand{not (OMem? o2)} -> cmp
+| Cmp_gt : o1:operand{not (OMem? o1)} -> o2:operand{not (OMem? o2)} -> cmp
 
 [@va_qattr]
 let cmp_to_ocmp (c:cmp) : ocmp =
@@ -177,11 +177,17 @@ let cmp_to_ocmp (c:cmp) : ocmp =
 let valid_cmp (c:cmp) (s:state) : Type0 =
   match c with
   | Cmp_eq o1 o2 -> valid_operand o1 s /\ valid_operand o2 s
+    /\ valid_taint o1 s Public /\ valid_taint o2 s Public
   | Cmp_ne o1 o2 -> valid_operand o1 s /\ valid_operand o2 s
+    /\ valid_taint o1 s Public /\ valid_taint o2 s Public
   | Cmp_le o1 o2 -> valid_operand o1 s /\ valid_operand o2 s
+    /\ valid_taint o1 s Public /\ valid_taint o2 s Public
   | Cmp_ge o1 o2 -> valid_operand o1 s /\ valid_operand o2 s
+    /\ valid_taint o1 s Public /\ valid_taint o2 s Public
   | Cmp_lt o1 o2 -> valid_operand o1 s /\ valid_operand o2 s
+    /\ valid_taint o1 s Public /\ valid_taint o2 s Public
   | Cmp_gt o1 o2 -> valid_operand o1 s /\ valid_operand o2 s
+    /\ valid_taint o1 s Public /\ valid_taint o2 s Public
 
 [@va_qattr]
 let eval_cmp (s:state) (c:cmp) : GTot bool =
@@ -196,7 +202,7 @@ let eval_cmp (s:state) (c:cmp) : GTot bool =
 [@va_qattr]
 let wp_If (#a:Type) (#c1:code) (#c2:code) (b:cmp) (qc1:quickCode a c1) (qc2:quickCode a c2) (s0:state) (k:state -> a -> Type0) : Type0 =
   // REVIEW: this duplicates k
-  valid_cmp b s0 /\ (eval_cmp s0 b ==> QProc?.wp qc1 s0 k) /\ (not (eval_cmp s0 b) ==> QProc?.wp qc2 s0 k)
+  valid_cmp b s0 /\ (eval_cmp s0 b ==> QProc?.wp qc1 ({s0 with trace=BranchPredicate(true)::s0.trace}) k) /\ (not (eval_cmp s0 b) ==> QProc?.wp qc2 ({s0 with trace=BranchPredicate(false)::s0.trace}) k)
 
 val qIf_monotone (#a:Type) (#c1:code) (#c2:code) (b:cmp) (qc1:quickCode a c1) (qc2:quickCode a c2) (s0:state) (k1:state -> a -> Type0) (k2:state -> a -> Type0) : Lemma
   (requires (forall (s:state) (g:a). k1 s g ==> k2 s g))
@@ -280,12 +286,14 @@ let va_state_match (s0:state) (s1:state) : Pure Type0
   all_regs_match s0.regs s1.regs /\
   all_xmms_match s0.xmms s1.xmms /\
   s0.flags == s1.flags /\
-  s0.mem == s1.mem
+  s0.mem == s1.mem /\
+  s0.trace == s1.trace /\
+  s0.memTaint == s1.memTaint
 
 [@va_qattr]
 unfold let wp_sound_pre (#a:Type0) (#cs:codes) (qcs:quickCodes a cs) (s0:state) (k:state -> state -> a -> Type0) : Type0 =
-  forall (ok:bool) (regs:Regs_i.t) (xmms:Xmms_i.t) (flags:nat64) (mem:mem).
-    let s0' = {ok = ok; regs = regs; xmms = xmms; flags = flags; mem = mem} in
+  forall (ok:bool) (regs:Regs_i.t) (xmms:Xmms_i.t) (flags:nat64) (mem:mem) (trace:list observation) (memTaint:map int taint).
+    let s0' = {ok = ok; regs = regs; xmms = xmms; flags = flags; mem = mem; trace=trace; memTaint=memTaint} in
     s0 == s0' ==> wp cs qcs (k s0') s0'
 
 unfold let wp_sound_post (#a:Type0) (#cs:codes) (qcs:quickCodes a cs) (s0:state) (k:state -> state -> a -> Type0) ((sN:state), (fN:fuel), (gN:a)) : Type0 =
@@ -299,8 +307,8 @@ val wp_sound_wrap (#a:Type0) (cs:codes) (qcs:quickCodes a cs) (s0:state) (k:stat
 
 [@va_qattr]
 unfold let wp_sound_code_pre (#a:Type0) (#c:code) (qc:quickCode a c) (s0:state) (k:state -> state -> a -> Type0) : Type0 =
-  forall (ok:bool) (regs:Regs_i.t) (xmms:Xmms_i.t) (flags:nat64) (mem:mem).
-    let s0' = {ok = ok; regs = regs; xmms = xmms; flags = flags; mem = mem} in
+  forall (ok:bool) (regs:Regs_i.t) (xmms:Xmms_i.t) (flags:nat64) (mem:mem) (trace:list observation) (memTaint:map int taint).
+    let s0' = {ok = ok; regs = regs; xmms = xmms; flags = flags; mem = mem; trace=trace; memTaint=memTaint} in
     s0 == s0' ==> QProc?.wp qc s0' (k s0')
 
 unfold let wp_sound_code_post (#a:Type0) (#c:code) (qc:quickCode a c) (s0:state) (k:state -> state -> a -> Type0) ((sN:state), (fN:fuel), (gN:a)) : Type0 =
@@ -318,21 +326,21 @@ val wp_sound_code_wrap (#a:Type0) (c:code) (qc:quickCode a c) (s0:state) (k:stat
 [@va_qattr]
 let wp_final_k (#a:Type0) (update:state -> state) (post:state -> state -> Type0) (k:state -> a -> Type0) (sN:state) (g:a) : Type0 =
   va_state_match sN (update sN) /\ post sN sN /\
-    (forall (ok':bool) (regs':Regs_i.t) (xmms':Xmms_i.t) (flags':nat64) (mem':mem).
-      let sN' = {ok = ok'; regs = regs'; xmms = xmms'; flags = flags'; mem = mem'} in
+    (forall (ok':bool) (regs':Regs_i.t) (xmms':Xmms_i.t) (flags':nat64) (mem':mem) (trace':list observation) (memTaint':map int taint).
+      let sN' = {ok = ok'; regs = regs'; xmms = xmms'; flags = flags'; mem = mem'; trace=trace'; memTaint=memTaint'} in
       post sN sN' ==> k sN' g)
 
 // For efficiency, introduce shorter names (e.g. ok, mem) for components of initial state s0.
 [@va_qattr]
 let wp_wrap (#a:Type0) (cs:codes) (qcs:quickCodes a cs) (update:state -> state -> state) (post:state -> state -> Type0) (k:state -> a -> Type0) (s0:state) : Type0 =
-  forall (ok:bool) (regs:Regs_i.t) (xmms:Xmms_i.t) (flags:nat64) (mem:mem).
-    let s0' = {ok = ok; regs = regs; xmms = xmms; flags = flags; mem = mem} in
+  forall (ok:bool) (regs:Regs_i.t) (xmms:Xmms_i.t) (flags:nat64) (mem:mem) (trace:list observation) (memTaint:map int taint).
+    let s0' = {ok = ok; regs = regs; xmms = xmms; flags = flags; mem = mem; trace=trace; memTaint=memTaint} in
     s0 == s0' ==> wp cs qcs (wp_final_k (update s0') post k) s0'
 
 [@va_qattr]
 let wp_wrap_code (#a:Type0) (c:code) (qc:quickCode a c) (update:state -> state -> state) (post:state -> state -> Type0) (k:state -> a -> Type0) (s0:state) : Type0 =
-  forall (ok:bool) (regs:Regs_i.t) (xmms:Xmms_i.t) (flags:nat64) (mem:mem).
-    let s0' = {ok = ok; regs = regs; xmms = xmms; flags = flags; mem = mem} in
+  forall (ok:bool) (regs:Regs_i.t) (xmms:Xmms_i.t) (flags:nat64) (mem:mem) (trace:list observation) (memTaint:map int taint).
+    let s0' = {ok = ok; regs = regs; xmms = xmms; flags = flags; mem = mem; trace=trace; memTaint=memTaint} in
     s0 == s0' ==> QProc?.wp qc s0' (wp_final_k (update s0') post k)
 
 unfold let wp_GHOST (#a:Type0) (c:code) (s0:state) (update:state -> state -> state) (fk:(state -> a -> Type0) -> Type0) (p:state * fuel * a -> Type0) : Type0 =
@@ -357,6 +365,8 @@ unfold let normal_steps : list string =
     "X64.Vale.State_i.__proj__Mkstate__item__xmms";
     "X64.Vale.State_i.__proj__Mkstate__item__flags";
     "X64.Vale.State_i.__proj__Mkstate__item__mem";
+    "X64.Vale.State_i.__proj__Mkstate__item__trace";
+    "X64.Vale.State_i.__proj__Mkstate__item__memTaint";    
 
     "X64.Vale.QuickCode_i.__proj__QProc__item__wp";
   ]
