src/arch/x64/X64.Vale.StateLemmas_i.fst
@@ -6,21 +6,26 @@ module M = TransparentMap
 module BS = X64.Bytes_Semantics_s
 module ME = X64.Memory_i_s
 module I = Interop64
+module TS = X64.Taint_Semantics_s
 
 #reset-options "--initial_fuel 2 --max_fuel 2"
 
-let state_to_S (s:state) : GTot ME.state = 
-  let s' = {
+let state_to_S (s:state) : GTot TS.traceState = 
+  {
+  TS.state = (let s' = {
     BS.ok = s.ok;
     BS.regs = (fun r -> s.regs r);
     BS.xmms = (fun x -> s.xmms x);
     BS.flags = int_to_nat64 s.flags;
     BS.mem = ME.get_heap s.mem
   } in
-  { ME.state = s'; ME.mem = s.mem}
+  { ME.state = s'; ME.mem = s.mem});
+  TS.trace = s.trace;
+  TS.memTaint = s.memTaint;
+  }
 
-let state_of_S (s:ME.state) : state =
-  let { ME.state = st; ME.mem = mem } = s in
+let state_of_S (s:TS.traceState) : state =
+  let { ME.state = st; ME.mem = mem } = s.TS.state in
   let { BS.ok = ok; BS.regs = regs; BS.xmms = xmms; BS.flags = flags; BS.mem = _} = st in
   {
     ok = ok;
@@ -28,6 +33,8 @@ let state_of_S (s:ME.state) : state =
     xmms = (fun x -> xmms x);
     flags = flags;
     mem = mem;
+    trace = s.TS.trace;
+    memTaint = s.TS.memTaint;
   }
 
 let lemma_to_ok s = ()
@@ -35,9 +42,12 @@ let lemma_to_flags s = ()
 let lemma_to_mem s = ()
 let lemma_to_reg s r = ()
 let lemma_to_xmm s x = ()
+let lemma_to_trace s = ()
+let lemma_to_memTaint s = ()
 let lemma_to_eval_operand s o = ()
 let lemma_to_eval_xmm s x = ()
 let lemma_to_valid_operand s o = ()
+let lemma_to_valid_taint s o t = ()
 
 let lemma_of_to s =
   assert (state_eq s (state_of_S (state_to_S s)));
@@ -46,11 +56,18 @@ let lemma_of_to s =
 let lemma_to_of s =
   let s' = state_of_S s in
   let s'' = state_to_S s' in
-  let { ME.state = st; ME.mem = mem } = s in
+  let { ME.state = st; ME.mem = mem } = s.TS.state in
   let { BS.ok = ok; BS.regs = regs; BS.xmms = xmms; BS.flags = flags; BS.mem = heap} = st in
-  let { ME.state = st''; ME.mem = mem'' } = s'' in
+  let { ME.state = st''; ME.mem = mem'' } = s''.TS.state in
   let { BS.ok = ok''; BS.regs = regs''; BS.xmms = xmms''; BS.flags = flags''; BS.mem = heap''} = st'' in
   assert (feq regs regs'');
   assert (feq xmms xmms'');
-  ME.same_heap s s'';
+  ME.same_heap s.TS.state s''.TS.state;
   ()
+
+let modify_trace s0 b =
+  let s1 = {s0 with trace = BranchPredicate(b)::s0.trace} in
+  let s0' = state_to_S s0 in
+  let s1' = state_to_S s1 in
+  assert (FunctionalExtensionality.feq s0'.TS.state.ME.state.BS.regs s1'.TS.state.ME.state.BS.regs);
+  assert (FunctionalExtensionality.feq s0'.TS.state.ME.state.BS.xmms s1'.TS.state.ME.state.BS.xmms)  
