src/arch/x64/X64.Vale.StateLemmas_i.fsti
@@ -6,53 +6,71 @@ module S = X64.Semantics_s
 module M = TransparentMap
 module BS = X64.Bytes_Semantics_s
 module ME = X64.Memory_i_s
+module TS = X64.Taint_Semantics_s
 
 unfold let ok' s = s.ME.state.BS.ok
 unfold let regs' s = s.ME.state.BS.regs
 unfold let xmms' s = s.ME.state.BS.xmms
 unfold let flags' s = s.ME.state.BS.flags
 unfold let mem' = ME.Mkstate'?.mem
+unfold let trace' = TS.MktraceState?.trace
+unfold let memTaint' = TS.MktraceState?.memTaint
 
-val state_to_S : s:state -> GTot ME.state
-val state_of_S : s:ME.state -> state
+val state_to_S : s:state -> GTot TS.traceState
+val state_of_S : s:TS.traceState -> state
 
 val lemma_to_ok : s:state -> Lemma
-  (ensures s.ok == ok' (state_to_S s))
+  (ensures s.ok == ok' (state_to_S s).TS.state)
   [SMTPat s.ok]
 
 val lemma_to_flags : s:state -> Lemma
-  (ensures s.flags == flags' (state_to_S s))
+  (ensures s.flags == flags' (state_to_S s).TS.state)
   [SMTPat s.flags]
 
 val lemma_to_mem : s:state -> Lemma
-  (ensures s.mem == mem' (state_to_S s))
+  (ensures s.mem == mem' (state_to_S s).TS.state)
   [SMTPat s.mem]
   
 val lemma_to_reg : s:state -> r:reg -> Lemma
-  (ensures s.regs r == regs' (state_to_S s) r)
+  (ensures s.regs r == regs' (state_to_S s).TS.state r)
   [SMTPat (s.regs r)]
 
 val lemma_to_xmm : s:state -> x:xmm -> Lemma
-  (ensures s.xmms x == xmms' (state_to_S s) x)
+  (ensures s.xmms x == xmms' (state_to_S s).TS.state x)
   [SMTPat (s.xmms x)]
 
+
+val lemma_to_trace : s:state -> Lemma
+  (ensures s.trace == trace' (state_to_S s))
+  [SMTPat s.trace]
+
+val lemma_to_memTaint : s:state -> Lemma
+  (ensures s.memTaint == memTaint' (state_to_S s))
+  [SMTPat s.memTaint]
+
 val lemma_to_eval_operand : s:state -> o:operand -> Lemma
-  (ensures eval_operand o s == S.eval_operand o (state_to_S s))
+  (ensures eval_operand o s == S.eval_operand o (state_to_S s).TS.state)
   [SMTPat (eval_operand o s)]
 
 val lemma_to_eval_xmm : s:state -> x:xmm -> Lemma
-  (ensures eval_xmm x s == S.eval_xmm x (state_to_S s))
+  (ensures eval_xmm x s == S.eval_xmm x (state_to_S s).TS.state)
   [SMTPat (eval_xmm x s)]
 
 val lemma_to_valid_operand : s:state -> o:operand -> Lemma
-  (ensures valid_operand o s ==> S.valid_operand o (state_to_S s))
+  (ensures valid_operand o s ==> S.valid_operand o (state_to_S s).TS.state)
   [SMTPat (valid_operand o s)]
+
+val lemma_to_valid_taint : s:state -> o:operand -> t:taint -> Lemma
+  (ensures valid_taint o s t ==> TS.taint_match o t (state_to_S s).TS.memTaint (state_to_S s).TS.state)
+  [SMTPat (valid_taint o s t)]
 
 val lemma_of_to : s:state -> Lemma
   (ensures s == state_of_S (state_to_S s))
   [SMTPat (state_of_S (state_to_S s))]
 
-val lemma_to_of : s:ME.state -> Lemma
+val lemma_to_of : s:TS.traceState -> Lemma
   (ensures s == state_to_S (state_of_S s))
   [SMTPat (state_to_S (state_of_S s))]
 
+val modify_trace: (s0:state) -> (b:bool) -> Lemma
+  (state_to_S ({s0 with trace=BranchPredicate(b)::s0.trace}) == ({(state_to_S s0) with TS.trace = BranchPredicate(b)::(state_to_S s0).TS.trace}))
